theories/ordinals/MoreAck/FolCoercions.v
@@ -350,7 +350,7 @@ Qed.
 (* begin snippet freeVarExamples *)
 Compute  freeVarFormula _ f2.
 
-Compute ListExt.no_dup _ Nat.eq_dec (freeVarFormula _ f3).
+Compute List.nodup Nat.eq_dec (freeVarFormula _ f3).
 
 Compute close _ f3.
 
